save

Superposition_Calculus/First_Order_Select.thy
@@ -2,6 +2,7 @@ theory First_Order_Select
   imports 
     Selection_Function
     First_Order_Clause
+    First_Order_Type_System
     HOL_Extra
 begin
 
@@ -15,34 +16,60 @@ definition is_select_grounding :: "('f, 'v) select \<Rightarrow> 'f ground_selec
         clause\<^sub>G = to_ground_clause (clause \<cdot> \<gamma>) \<and> 
         select\<^sub>G clause\<^sub>G = to_ground_clause ((select clause) \<cdot> \<gamma>))"
 
+definition typed_clause_groundings where
+  "typed_clause_groundings \<F> clause = { to_ground_clause (clause \<cdot> \<gamma>) | \<gamma>. 
+    is_ground_clause (clause \<cdot> \<gamma>) \<and> (\<forall>\<V>. welltyped\<^sub>c \<F> \<V> clause \<longleftrightarrow> welltyped\<^sub>c \<F> \<V> (clause \<cdot> \<gamma>))
+}"
+
 (* TODO: Factor out sth like select_subst_stable for a single premise and use that format 
   everywhere *)
 abbreviation select_subst_stability_on where
-  "\<And>select select\<^sub>G. select_subst_stability_on select select\<^sub>G premises \<equiv>
-    \<forall>premise\<^sub>G \<in> \<Union> (clause_groundings ` premises). \<exists>premise \<in> premises. \<exists>\<gamma>. 
+  "\<And>select select\<^sub>G. select_subst_stability_on \<F> select select\<^sub>G premises \<equiv>
+    \<forall>premise\<^sub>G \<in> \<Union> (clause_groundings ` premises). \<exists>premise \<in> premises. \<exists>\<gamma> \<V>. 
       premise \<cdot> \<gamma> = to_clause premise\<^sub>G \<and> 
-      select\<^sub>G (to_ground_clause (premise \<cdot> \<gamma>)) = to_ground_clause ((select premise) \<cdot> \<gamma>)"
+      select\<^sub>G (to_ground_clause (premise \<cdot> \<gamma>)) = to_ground_clause ((select premise) \<cdot> \<gamma>) \<and>
+      (welltyped\<^sub>c \<F> \<V> (premise \<cdot> \<gamma>) \<longleftrightarrow> welltyped\<^sub>c \<F> \<V> premise)"
+
+abbreviation typed_select_subst_stability_on where
+  "\<And>select select\<^sub>G. typed_select_subst_stability_on \<F> select select\<^sub>G premises \<equiv>
+    \<forall>premise\<^sub>G \<in> \<Union> (typed_clause_groundings \<F> ` premises). \<exists>premise \<in> premises. \<exists>\<gamma> \<V>. 
+      premise \<cdot> \<gamma> = to_clause premise\<^sub>G \<and> 
+      select\<^sub>G (to_ground_clause (premise \<cdot> \<gamma>)) = to_ground_clause ((select premise) \<cdot> \<gamma>) \<and>
+       (welltyped\<^sub>c \<F> \<V> (premise \<cdot> \<gamma>) \<longleftrightarrow> welltyped\<^sub>c \<F> \<V> premise)"
+
+(*lemma welltyped\<^sub>c_grounding:
+  assumes "premise \<cdot> \<gamma> = to_clause premise\<^sub>G"
+  shows "\<exists>\<V>. welltyped\<^sub>c \<F> \<V> premise \<longrightarrow> welltyped\<^sub>\<sigma> \<F> \<V> \<gamma>"
+  sorry*)
+
+(*lemma welltyped\<^sub>c_grounding:
+  assumes "premise \<cdot> \<gamma> = to_clause premise\<^sub>G" "welltyped\<^sub>c \<F> \<V> premise" 
+  shows "welltyped\<^sub>\<sigma> \<F> \<V> \<gamma>"
+  sorry*)
 
 lemma obtain_subst_stable_on_select_grounding:
   fixes select :: "('f, 'v) select"
   obtains select\<^sub>G where 
-    "select_subst_stability_on select select\<^sub>G premises"
+    "typed_select_subst_stability_on \<F> select select\<^sub>G premises"
     "is_select_grounding select select\<^sub>G"
 proof-
-  let ?premise_groundings = "\<Union>(clause_groundings ` premises)"
+  let ?premise_groundings = "\<Union>(typed_clause_groundings \<F> ` premises)"
 
   have select\<^sub>G_exists_for_premises: 
-    "\<forall>premise\<^sub>G \<in> ?premise_groundings. \<exists>select\<^sub>G \<gamma>. \<exists>premise \<in> premises.
+    "\<forall>premise\<^sub>G \<in> ?premise_groundings. \<exists>select\<^sub>G \<gamma> \<V>. \<exists>premise \<in> premises.
           premise \<cdot> \<gamma> = to_clause premise\<^sub>G 
-        \<and> select\<^sub>G premise\<^sub>G = to_ground_clause ((select premise) \<cdot> \<gamma>)"
-    unfolding clause_groundings_def
+        \<and> select\<^sub>G premise\<^sub>G = to_ground_clause ((select premise) \<cdot> \<gamma>) \<and>
+         (welltyped\<^sub>c \<F> \<V> (premise \<cdot> \<gamma>) \<longleftrightarrow> welltyped\<^sub>c \<F> \<V> premise)"
+    unfolding typed_clause_groundings_def
     by fastforce
 
   obtain select\<^sub>G_on_premise_groundings where 
-    select\<^sub>G_on_premise_groundings: "\<forall>premise\<^sub>G \<in>?premise_groundings. \<exists>premise \<in> premises. \<exists>\<gamma>.
+    select\<^sub>G_on_premise_groundings: "\<forall>premise\<^sub>G \<in>?premise_groundings. \<exists>premise \<in> premises. \<exists>\<gamma> \<V>.
         premise \<cdot> \<gamma> = to_clause premise\<^sub>G 
       \<and> select\<^sub>G_on_premise_groundings (to_ground_clause (premise \<cdot> \<gamma>)) = 
-          to_ground_clause ((select premise) \<cdot> \<gamma>)"
+          to_ground_clause ((select premise) \<cdot> \<gamma>)
+      \<and> (welltyped\<^sub>c \<F> \<V> (premise \<cdot> \<gamma>) \<longrightarrow> welltyped\<^sub>c \<F> \<V> premise) \<and> 
+        (\<not> welltyped\<^sub>c \<F> \<V> (premise \<cdot> \<gamma>) \<longrightarrow> \<not> welltyped\<^sub>c \<F> \<V> premise)"
     using Ball_Ex_comm(1)[OF select\<^sub>G_exists_for_premises]
     by (metis (mono_tags, opaque_lifting) to_clause_inverse)
 
@@ -59,7 +86,6 @@ proof-
     by (metis ground_clause_is_ground subst_clause_Var_ident to_clause_inverse)
 
   show ?thesis
-    
     using that[OF _ grounding] select\<^sub>G_on_premise_groundings
     unfolding select\<^sub>G_def 
     by fastforce
@@ -129,7 +155,10 @@ locale grounded_first_order_select =
 begin
 
 abbreviation subst_stability_on where
-  "subst_stability_on premises \<equiv> select_subst_stability_on select select\<^sub>G premises"
+  "subst_stability_on \<F> premises \<equiv> select_subst_stability_on \<F> select select\<^sub>G premises"
+
+abbreviation typed_subst_stability_on where
+  "typed_subst_stability_on \<F> premises \<equiv> typed_select_subst_stability_on \<F> select select\<^sub>G premises"
   
 lemma select\<^sub>G_subset: "select\<^sub>G clause \<subseteq># clause"
   using select\<^sub>G 
